doc/changelog/10-standard-library/14384-Sint63_additions.rst
@@ -1,0 +1,4 @@
+- **Added:**
+  Absolute value function for Sint63.
+  (`#14384 <https://github.com/coq/coq/pull/14384>`_,
+  by Ana Borges).
